theories/LRInduction.v
@@ -9,8 +9,8 @@ Section Inductions.
     `{!ConvType ta} `{!ConvTerm ta} `{!ConvNeuConv ta}
     `{!RedType ta} `{!RedTerm ta}.
 
-  Fixpoint LR_embedding@{i j k} {l l'} (l_ : l << l')
-    {Γ A rEq rTe rTeEq} (lr : LogRel@{i j k} l Γ A rEq rTe rTeEq) {struct lr} : (LogRel@{i j k} l' Γ A rEq rTe rTeEq) :=
+  Fixpoint LR_embedding@{i j k l} {l l'} (l_ : l << l')
+    {Γ A rEq rTe rTeEq} (lr : LogRel@{i j k l} l Γ A rEq rTe rTeEq) {struct lr} : (LogRel@{i j k l} l' Γ A rEq rTe rTeEq) :=
     match lr with
     | LRU _ H =>
         match
@@ -90,9 +90,9 @@ Section Inductions.
     now apply LR_rect.
   Qed.
 
-  Theorem LR_rect_LogRelRec@{i j k o}
+  Theorem LR_rect_LogRelRec@{i j k l o}
     (P : forall {l Γ t rEq rTe rTeEq},
-    LogRel@{i j k} l Γ t rEq rTe rTeEq -> Type@{o}) :
+    LogRel@{i j k l} l Γ t rEq rTe rTeEq -> Type@{o}) :
 
     (forall (Γ : context) (h : [Γ ||-U one]),
       P (LRU (rec1) h)) ->
@@ -109,12 +109,12 @@ Section Inductions.
     P (HAad.(PiRedTy.codAd) ρ h ha)) ->
     P (LRPi (LogRelRec l) ΠA HAad)) ->
 
-    forall (l : TypeLevel) (Γ : context) (t : term) (rEq rTe : term -> Type@{j})
-      (rTeEq  : term -> term -> Type@{j}) (lr : LR@{i j k} (LogRelRec@{i j} l) Γ t rEq rTe rTeEq),
+    forall (l : TypeLevel) (Γ : context) (t : term) (rEq rTe : term -> Type@{k})
+      (rTeEq  : term -> term -> Type@{k}) (lr : LR@{j k l} (LogRelRec@{i j k} l) Γ t rEq rTe rTeEq),
       P lr.
   Proof.
     intros.
-    apply LR_rect@{i j k o}.
+    apply LR_rect@{j k l o}.
     - intros.
       destruct l.
       2: auto.
@@ -124,8 +124,8 @@ Section Inductions.
     - auto.
   Qed.
 
-  Theorem LR_rect_TyUr@{i j k o}
-    (P : forall {l Γ A}, [LogRel@{i j k} l | Γ ||- A] -> Type@{o}) :
+  Theorem LR_rect_TyUr@{i j k l o }
+    (P : forall {l Γ A}, [LogRel@{i j k l} l | Γ ||- A] -> Type@{o}) :
 
     (forall (Γ : context) (h : [Γ ||-U one]),
       P (LRU_ h)) ->
@@ -141,26 +141,24 @@ Section Inductions.
     P (LRbuild (HAad.(PiRedTy.codAd) ρ h ha))) ->
     P (LRPi_ l ΠA HAad)) ->
 
-    forall (l : TypeLevel) (Γ : context) (A : term) (lr : [LogRel@{i j k} l | Γ ||- A]),
+    forall (l : TypeLevel) (Γ : context) (A : term) (lr : [LogRel@{i j k l} l | Γ ||- A]),
       P lr.
   Proof.
     intros HU Hne HPi l Γ A lr.
-    apply (LR_rect_LogRelRec (fun l Γ A _ _ _ lr => P l Γ A (LRbuild lr))).
+    apply (LR_rect_LogRelRec@{i j k l o} (fun l Γ A _ _ _ lr => P l Γ A (LRbuild lr))).
     all: auto.
   Qed.
 
   (* Induction principle specialized at level 0 to minimize universe constraints *)
-  Theorem LR_rect0@{i j o}
+  (* Useful anywhere ? *)
+  Theorem LR_rect0@{i j k o}
     (P : forall {c t rEq rTe rTeEq},
-      LogRel0@{i j} c t rEq rTe rTeEq  -> Type@{o}) :
-
-    (* (forall (Γ : context) (h : [Γ ||-U zero]), *)
-    (*   P (LRU rec0 h)) -> *)
+      LogRel0@{i j k} c t rEq rTe rTeEq  -> Type@{o}) :
 
     (forall (Γ : context) (A : term) (neA : [Γ ||-ne A]),
       P (LRne rec0 neA)) -> 
 
-    (forall (Γ : context) (A : term) (ΠA : [ Γ ||-Πd A ]) (HAad : PiRedTyAdequate (LogRel0@{i j}) ΠA),
+    (forall (Γ : context) (A : term) (ΠA : [ Γ ||-Πd A ]) (HAad : PiRedTyAdequate (LogRel0@{i j k}) ΠA),
     (forall {Δ} (ρ : Δ ≤ Γ) (h : [ |- Δ]),
       P (HAad.(PiRedTy.domAd) ρ h)) ->
     (forall {Δ a} (ρ : Δ ≤ Γ) (h : [ |- Δ ]) 
@@ -168,12 +166,12 @@ Section Inductions.
     P (HAad.(PiRedTy.codAd) ρ h ha)) ->
     P (LRPi rec0 ΠA HAad)) ->
 
-    forall (Γ : context) (t : term) (rEq rTe : term -> Type@{i})
-      (rTeEq  : term -> term -> Type@{i}) (lr : LogRel0@{i j} Γ t rEq rTe rTeEq),
+    forall (Γ : context) (t : term) (rEq rTe : term -> Type@{j})
+      (rTeEq  : term -> term -> Type@{j}) (lr : LogRel0@{i j k} Γ t rEq rTe rTeEq),
       P lr.
   Proof.
     cbn.
-    intros (* HU *) Hne HPi.
+    intros Hne HPi.
     fix HRec 6.
     destruct lr.
     - destruct H as [? lt]; destruct (elim lt).
@@ -182,27 +180,24 @@ Section Inductions.
       all: intros ; eapply HRec.
   Qed.
 
-  Theorem LR_rect_TyUr0@{i j o}
-    (P : forall {Γ A}, [LogRel0@{i j} | Γ ||- A] -> Type@{o}) :
-
-    (* (forall (Γ : context) (h : [Γ ||-U zero]), *)
-    (*   P (LRU_ h)) -> *)
+  Theorem LR_rect_TyUr0@{i j k o}
+    (P : forall {Γ A}, [LogRel0@{i j k} | Γ ||- A] -> Type@{o}) :
 
     (forall (Γ : context) (A : term) (neA : [Γ ||-ne A]),
-      P (LRbuild0@{i j} (LRne@{Set i j} rec0 neA))) ->
+      P (LRbuild0@{i j k} (LRne@{i j k} rec0 neA))) ->
 
     (forall (Γ : context) (A : term) (ΠA : [ Γ ||-Πd A ]) (HAad : PiRedTyAdequate LogRel0 ΠA),
     (forall {Δ} (ρ : Δ ≤ Γ) (h : [ |- Δ]),
-      P (LRbuild0@{i j} (HAad.(PiRedTy.domAd) ρ h))) ->
+      P (LRbuild0@{i j k} (HAad.(PiRedTy.domAd) ρ h))) ->
     (forall {Δ a} (ρ : Δ ≤ Γ) (h : [ |- Δ ]) 
       (ha : [ ΠA.(PiRedTy.domRed) ρ h | Δ ||- a : ΠA.(PiRedTy.dom)⟨ρ⟩ ]),
-    P (LRbuild0@{i j} (HAad.(PiRedTy.codAd) ρ h ha))) ->
-    P (LRbuild0@{i j} (LRPi rec0 ΠA HAad))) ->
+    P (LRbuild0@{i j k} (HAad.(PiRedTy.codAd) ρ h ha))) ->
+    P (LRbuild0@{i j k} (LRPi rec0 ΠA HAad))) ->
 
-    forall (Γ : context) (A : term) (lr : [LogRel0@{i j} | Γ ||- A]),
+    forall (Γ : context) (A : term) (lr : [LogRel0@{i j k} | Γ ||- A]),
       P lr.
   Proof.
-    intros (* HU *) Hne HPi Γ A lr.
+    intros Hne HPi Γ A lr.
     apply (LR_rect0 (fun Γ A _ _ _ lr => P Γ A (LRbuild0 lr))).
     all: auto.
   Qed.
